Improve performance of sum type definitions (with @nikswamy)

src/lowparse/LowParseExample.Aux.fst
@@ -19,17 +19,44 @@ noeq
 type t =
   | A of (U8.t * U8.t)
   | B of case_B
+  | V2 of U16.t
+  | V3 of U16.t
+  | V4 of U16.t
+  | V5 of U16.t
+  | V6 of U16.t
+  | V7 of U16.t
+  | V8 of U16.t
+  | V9 of U16.t
 
 type cases : eqtype =
   | Case_A
   | Case_B
+  | Case_V2
+  | Case_V3
+  | Case_V4
+  | Case_V5
+  | Case_V6
+  | Case_V7
+  | Case_V8
+  | Case_V9
 
 inline_for_extraction
-let case_enum : LP.enum cases U8.t =
+let u8 : eqtype = U8.t
+
+inline_for_extraction
+let case_enum : LP.enum cases u8 =
   [@inline_let]
   let e : list (cases * U8.t) = [
     Case_A, 18uy;
     Case_B, 42uy;
+    Case_V2, 71uy;
+    Case_V3, 72uy;
+    Case_V4, 73uy;
+    Case_V5, 74uy;
+    Case_V6, 75uy;
+    Case_V7, 76uy;
+    Case_V8, 77uy;
+    Case_V9, 78uy;
   ]
   in
   [@inline_let]
@@ -39,13 +66,35 @@ let case_enum : LP.enum cases U8.t =
   in
   e
 
+// #reset-options "--using_facts_from '* -FStar.Tactics -FStar.Reflection' --z3rlimit 16 --z3cliopt smt.arith.nl=false --max_fuel 2 --max_ifuel 2 --query_stats --z3refresh"
+
+// #set-options "--debug_level SMTQuery --debug LowParseExample.Aux --print_full_names"
+
+// NOTE: this coercion is necessary otherwise cases_of_t does not typecheck for large sum types. In fact, the return value of cases_of_t is LP.enum_key case_enum instead of cases (i.e. the enum is not necessarily total)
+
+inline_for_extraction
+unfold
+let case_as_case_enum
+  (x: cases { norm [delta; zeta; iota; primops] (LP.list_mem x (LP.list_map fst case_enum)) == true } )
+: Tot (LP.enum_key case_enum)
+= norm_spec [delta; zeta; iota; primops] (LP.list_mem x (LP.list_map fst case_enum));
+  x
+
 inline_for_extraction
 let cases_of_t
   (x: t)
-: Tot cases
+: Tot (LP.enum_key case_enum)
 = match x with
-  | A _ -> Case_A
-  | B _ -> Case_B
+  | A _ -> case_as_case_enum Case_A
+  | B _ -> case_as_case_enum Case_B
+  | V2 _ -> case_as_case_enum Case_V2
+  | V3 _ -> case_as_case_enum Case_V3
+  | V4 _ -> case_as_case_enum Case_V4
+  | V5 _ -> case_as_case_enum Case_V5
+  | V6 _ -> case_as_case_enum Case_V6
+  | V7 _ -> case_as_case_enum Case_V7
+  | V8 _ -> case_as_case_enum Case_V8
+  | V9 _ -> case_as_case_enum Case_V9
 
 inline_for_extraction
 let type_of_case
@@ -54,24 +103,122 @@ let type_of_case
 = match x with
   | Case_A -> U8.t * U8.t
   | Case_B -> case_B
+  | Case_V2 -> U16.t
+  | Case_V3 -> U16.t
+  | Case_V4 -> U16.t
+  | Case_V5 -> U16.t
+  | Case_V6 -> U16.t
+  | Case_V7 -> U16.t
+  | Case_V8 -> U16.t
+  | Case_V9 -> U16.t
+
+// BEGIN typechecking performance improvements thanks to normalization and tactics
+
+unfold
+inline_for_extraction
+let to_type_of_case
+  (x: cases)
+  (#x' : cases)
+  (y: type_of_case x')
+: Pure (norm [delta_only [(`%type_of_case)]; iota] (type_of_case x))
+  (requires (x == x'))
+  (ensures (fun y' -> y' == y))
+= norm_spec [delta_only [(`%type_of_case)] ; iota] (type_of_case x);
+  y
+
+unfold
+inline_for_extraction
+let to_refine_with_tag (k: LP.enum_key case_enum) (x: t) : Pure (LP.refine_with_tag cases_of_t k)
+  (requires (
+    norm [delta; iota; zeta] (cases_of_t x) == k
+  ))
+  (ensures (fun y -> y == x))
+= norm_spec [delta; iota; zeta] (cases_of_t x);
+  x
 
 inline_for_extraction
 let synth_case
-  (x: cases)
+  (x: LP.enum_key case_enum)
   (y: type_of_case x)
 : Tot (LP.refine_with_tag cases_of_t x)
 = match x with
-  | Case_A -> A y
-  | Case_B -> B y
+  | Case_A -> to_refine_with_tag x (A (to_type_of_case Case_A y))
+  | Case_B -> to_refine_with_tag x (B (to_type_of_case Case_B y))
+  | Case_V2 -> to_refine_with_tag x (V2 (to_type_of_case Case_V2 y))
+  | Case_V3 -> to_refine_with_tag x (V3 (to_type_of_case Case_V3 y))
+  | Case_V4 -> to_refine_with_tag x (V4 (to_type_of_case Case_V4 y))
+  | Case_V5 -> to_refine_with_tag x (V5 (to_type_of_case Case_V5 y))
+  | Case_V6 -> to_refine_with_tag x (V6 (to_type_of_case Case_V6 y))
+  | Case_V7 -> to_refine_with_tag x (V7 (to_type_of_case Case_V7 y))
+  | Case_V8 -> to_refine_with_tag x (V8 (to_type_of_case Case_V8 y))
+  | Case_V9 -> to_refine_with_tag x (V9 (to_type_of_case Case_V9 y))
+
+unfold
+inline_for_extraction
+let from_type_of_case
+  (#x' : cases)
+  (x: cases)
+  (y: norm [delta_only [(`%type_of_case)]; iota] (type_of_case x))
+: Pure (type_of_case x')
+  (requires (x == x'))
+  (ensures (fun y' -> y' == y))
+= norm_spec [delta_only [(`%type_of_case)] ; iota] (type_of_case x);
+  y
+
+inline_for_extraction
+let synth_case_recip_pre
+  (k: LP.enum_key case_enum)
+  (x: LP.refine_with_tag cases_of_t k)
+: GTot bool
+= match k with
+  | Case_A -> (A? x)
+  | Case_B -> (B? x)
+  | Case_V2 -> (V2? x)
+  | Case_V3 -> (V3? x)
+  | Case_V4 -> (V4? x)
+  | Case_V5 -> (V5? x)
+  | Case_V6 -> (V6? x)
+  | Case_V7 -> (V7? x)
+  | Case_V8 -> (V8? x)
+  | Case_V9 -> (V9? x)
+
+module T = LowParse.TacLib
+
+let synth_case_recip_pre_intro1
+  (k: LP.enum_key case_enum)
+: Tot (
+  (x: t) ->
+  Tot (squash (k == cases_of_t x ==> synth_case_recip_pre k x == true)))
+= _ by (LP.synth_case_recip_pre_tac ())
+
+let synth_case_recip_pre_intro
+  (k: LP.enum_key case_enum)
+  (x: LP.refine_with_tag cases_of_t k)
+: Lemma (synth_case_recip_pre k x == true)
+= norm_spec [delta; iota] (synth_case_recip_pre k x);
+  assert (k == cases_of_t x);
+  let _ = synth_case_recip_pre_intro1 k x in
+  assert (k == cases_of_t x ==> synth_case_recip_pre k x == true); // FIXME: this is a BUG in F*, this assert should not be needed
+  ()
 
 inline_for_extraction
 let synth_case_recip
-  (k: cases)
+  (k: LP.enum_key case_enum)
   (x: LP.refine_with_tag cases_of_t k)
 : Tot (type_of_case k)
 = match k with
-  | Case_A -> (match x with A y -> (y <: type_of_case k))
-  | Case_B -> (match x with B y -> (y <: type_of_case k))
+  | Case_A -> synth_case_recip_pre_intro Case_A x; (match x with A y -> (from_type_of_case Case_A y))
+  | Case_B -> synth_case_recip_pre_intro Case_B x;(match x with B y -> (from_type_of_case Case_B y))
+  | Case_V2 -> synth_case_recip_pre_intro Case_V2 x;(match x with V2 y -> (from_type_of_case Case_V2 y))
+  | Case_V3 -> synth_case_recip_pre_intro Case_V3 x; (match x with V3 y -> (from_type_of_case Case_V3 y))
+  | Case_V4 -> synth_case_recip_pre_intro Case_V4 x; (match x with V4 y -> (from_type_of_case Case_V4 y))
+  | Case_V5 -> synth_case_recip_pre_intro Case_V5 x; (match x with V5 y -> (from_type_of_case Case_V5 y))
+  | Case_V6 -> synth_case_recip_pre_intro Case_V6 x; (match x with V6 y -> (from_type_of_case Case_V6 y))
+  | Case_V7 -> synth_case_recip_pre_intro Case_V7 x; (match x with V7 y -> (from_type_of_case Case_V7 y))
+  | Case_V8 -> synth_case_recip_pre_intro Case_V8 x; (match x with V8 y -> (from_type_of_case Case_V8 y))
+  | Case_V9 -> synth_case_recip_pre_intro Case_V9 x; (match x with V9 y -> (from_type_of_case Case_V9 y))
+
+// END typechecking performance improvements
 
 inline_for_extraction
 let t_sum : LP.sum
@@ -86,6 +233,7 @@ let parse_cases
 = match x with
   | Case_A -> (| _, LP.parse_u8 `LP.nondep_then` LP.parse_u8 |)
   | Case_B -> (| _, parse_case_B |)
+  | _ -> (| _, LP.parse_u16 |)
 
 let parse32_case_B : LP.parser32 parse_case_B =
   LP.parse32_filter LP.parse32_u16 parse_case_B_filter (fun x -> U16.gt x 0us)
@@ -97,6 +245,7 @@ let parse32_cases
 = match x with
   | Case_A -> (LP.parse32_nondep_then LP.parse32_u8 LP.parse32_u8 <: LP.parser32 (dsnd (parse_cases x)))
   | Case_B -> (parse32_case_B <: LP.parser32 (dsnd (parse_cases x)))
+  | _ -> (LP.parse32_u16 <: LP.parser32 (dsnd (parse_cases x)))
 
 let parse_t : LP.parser _ t =
   LP.parse_sum t_sum LP.parse_u8 parse_cases
@@ -127,6 +276,7 @@ let serialize_cases
 = match x with
   | Case_A -> (LP.serialize_nondep_then _ LP.serialize_u8 () _ LP.serialize_u8 <: LP.serializer (dsnd (parse_cases x)))
   | Case_B -> (serialize_case_B <: LP.serializer (dsnd (parse_cases x)))
+  | _ -> (LP.serialize_u16 <: LP.serializer (dsnd (parse_cases x)))
 
 inline_for_extraction
 let serialize32_cases
@@ -135,6 +285,7 @@ let serialize32_cases
 = match x with
   | Case_A -> (LP.serialize32_nondep_then LP.serialize32_u8 () LP.serialize32_u8 () <: LP.serializer32 (serialize_cases x))
   | Case_B -> (serialize32_case_B <: LP.serializer32 (serialize_cases x))
+  | _ -> (LP.serialize32_u16 <: LP.serializer32 (serialize_cases x))
 
 let serialize_t : LP.serializer parse_t =
   LP.serialize_sum t_sum LP.serialize_u8 serialize_cases
@@ -169,6 +320,7 @@ let size32_cases
 = match x with
   | Case_A -> (LP.size32_nondep_then LP.size32_u8 () LP.size32_u8 <: LP.size32 (serialize_cases x))
   | Case_B -> (size32_case_B <: LP.size32 (serialize_cases x))
+  | _ -> (LP.size32_u16 <: LP.size32 (serialize_cases x))
 
 let size32_t : LP.size32 serialize_t =
   assert_norm (LP.size32_sum_gen_precond (LP.get_parser_kind LP.parse_u8) (LP.weaken_parse_cases_kind t_sum parse_cases));
